\begin{lemma}
\label{lem:1-2vs1:ortho-lower-bound}
If there are $N < j \leq Q-N$ and $\lambda \in \indexSet{N}$ s.t. $L(x_{2j-\lambda}, y_j) = \rho_0$, we have
\[ 
L(x,y) \geq Q\Gamma + (Q-N)\ell_y + (N-1)\rho_1 + \rho_0.
\]
We define $i := 2j - \lambda$, i.e., $L(x_i, y_j) = \rho_0$.
\end{lemma}

\begin{proof}
Assume such $j$ and $\lambda$ exist.
We split the strings $x$ and $y$ into the three parts
\begin{align*}
x = \lLCSGadget{x_1, \ldots, x_P} &= \lLCSGadget{x^L_1, \ldots, x^L_{P'}} \lLCSGadget{x^M_1, \ldots, x^M_N} \lLCSGadget{x^R_1, \ldots, x^R_{P''}} =: \lLCSGadgetName^L_x\lLCSGadgetName^M_x\lLCSGadgetName^R_x \quad\text{and}\\
y = \lLCSGadget{y_1, \ldots, y_Q} &= \lLCSGadget{y^L_1, \ldots, y^L_{Q'}} \lLCSGadget{y^M_1, \ldots, y^M_N} \lLCSGadget{y^R_1, \ldots, y^R_{Q''}} =: \lLCSGadgetName^L_y\lLCSGadgetName^M_y\lLCSGadgetName^R_y,
\end{align*}
where $Q' = j - \lambda$, $P' = 2(j - \lambda)$, $Q'' = Q - Q' - N$ and $P'' = P - P' - N$.
We now want to lower bound the three parts. %$L^L := L(\lLCSGadgetName^L_x, \lLCSGadgetName^L_y)$, $L^M := L(\lLCSGadgetName^M_x, \lLCSGadgetName^M_y)$ and $L^R := L(\lLCSGadgetName^R_x, \lLCSGadgetName^R_y)$.
For the left and right part, note that $P' = 2Q'$ and $P'' = 2Q''$, hence we can apply \autoref{lem:1-2vs1-gadget-edge-cases} (\ref{lem:1-2vs1-gadget-edge-cases:P=2Q}) to have
\begin{align*}
L(\lLCSGadgetName^L_x, \lLCSGadgetName^L_y) &\geq Q'(\Gamma + \ell_y) \\
L(\lLCSGadgetName^R_x, \lLCSGadgetName^R_y) &\geq Q''(\Gamma + \ell_y) = (Q - Q' - N)(\Gamma + \ell_y).
\end{align*}
For the middle part, we first show that $x_i$ and $y_j$ are in the middle part, i.e., $x_i = x^M_{i'}$ and $y_j = y^M_{j'}$ for some $i', j' \in \indexSet{N}$.
Note therefore that
\begin{align*}
P' = 2j - 2\lambda &<& &2j - \lambda = i& &\leq 2j - \lambda - \lambda + N = P' + N \quad\text{and}\\
Q' = j - \lambda &<& &j& &\leq j - \lambda + N = Q' + N,
\end{align*}
where we used $1 \leq \lambda \leq N$.
Now we can apply \autoref{lem:1-2vs1-gadget-edge-cases} (\ref{lem:1-2vs1-gadget-edge-cases:P=Q}) with $P=Q=N$ and use the fact that $L(x^M_{i'}, y^M_{j'}) = L(x_i, y_j) = \rho_0$ to bound
\[
L(\lLCSGadgetName^M_x, \lLCSGadgetName^M_y) \geq N\Gamma + \sum_{k=1}^N L(x^M_k, y^M_k) \geq N\Gamma + (N-1)\rho_1 + \rho_0,
\]
where we used that $L(x^M_k, y^M_k) \geq \rho_1$ for all $k \in \indexSet{N}$.
Finally, we obtain
\begin{align*}
L(x,y) &\geq L(\lLCSGadgetName^L_x, \lLCSGadgetName^L_y) + L(\lLCSGadgetName^M_x, \lLCSGadgetName^M_y) + L(\lLCSGadgetName^R_x, \lLCSGadgetName^R_y)\\
	&\geq Q'(\Gamma + \ell_y) + N\Gamma + (N-1)\rho_1 + \rho_0 + (Q - Q' - N)(\Gamma + \ell_y) \\
	&= Q\Gamma + (Q-N)\ell_y + (N-1)\rho_1 + \rho_0,
\end{align*}
which is the desired bound.
\end{proof}
